Verify IAM helper functions that involve loop

src/proof/iam_model/common.v
@@ -1,4 +1,6 @@
 From New.proof Require Import prelude empty_ffi.
+From New.proof Require Import external_wp.
+From New.proof.map Require Import for_range.
 From New.proof.iam_model Require Export iammodel_init.
 From New.proof.iam_model Require Export inv.
 
@@ -39,6 +41,168 @@ Proof.
   constructor. iIntros (stk E Ψ) "HΨ". wp_auto. done.
 Qed.
 
+Lemma is_pkg_init_errors_trivial :
+  ⊢ (is_pkg_init errors : iProp Σ).
+Proof.
+  iEval (rewrite is_pkg_init_unfold /=). iSplit; iModIntro; done.
+Qed.
+
+Lemma is_pkg_init_race_trivial :
+  ⊢ (is_pkg_init race : iProp Σ).
+Proof.
+  iEval (rewrite is_pkg_init_unfold /=). iSplit; iModIntro; done.
+Qed.
+
+Lemma is_pkg_init_synctest_trivial :
+  ⊢ (is_pkg_init synctest : iProp Σ).
+Proof.
+  iEval (rewrite is_pkg_init_unfold /=). iSplit; iModIntro; done.
+Qed.
+
+Lemma is_pkg_init_atomic_trivial :
+  ⊢ (is_pkg_init atomic : iProp Σ).
+Proof.
+  iEval (rewrite is_pkg_init_unfold /=). iSplit; iModIntro; done.
+Qed.
+
+Lemma is_pkg_init_sync_trivial :
+  ⊢ (is_pkg_init sync : iProp Σ).
+Proof.
+  iEval (rewrite is_pkg_init_unfold /=).
+  iSplit.
+  - iModIntro. iSplit; [iApply is_pkg_init_synctest_trivial|].
+    iSplit; [iApply is_pkg_init_race_trivial|].
+    iSplit; [iApply is_pkg_init_atomic_trivial|done].
+  - iModIntro. done.
+Qed.
+
+Lemma is_pkg_init_io_trivial :
+  ⊢ (is_pkg_init io : iProp Σ).
+Proof.
+  iEval (rewrite is_pkg_init_unfold /=).
+  iSplit.
+  - iModIntro. iSplit; [iApply is_pkg_init_errors_trivial|].
+    iSplit; [iApply is_pkg_init_sync_trivial|done].
+  - iModIntro. done.
+Qed.
+
+Lemma is_pkg_init_fmt_trivial :
+  ⊢ (is_pkg_init fmt : iProp Σ).
+Proof.
+  iEval (rewrite is_pkg_init_unfold /=).
+  iSplit.
+  - iModIntro. iSplit; [iApply is_pkg_init_io_trivial|done].
+  - iModIntro. done.
+Qed.
+
+Definition processed_map `{Countable K} {A}
+    (keys : list K) (i : Z) (m : gmap K A) : gmap K A :=
+  filter (λ '(k, _), k ∈ list_to_set (C:=gset K) (take (Z.to_nat i) keys)) m.
+
+Lemma current_key_not_in_take `{EqDecision A} `{Countable A} (keys : list A) i key :
+  NoDup keys →
+  keys !! Z.to_nat i = Some key →
+  (0 ≤ i)%Z →
+  key ∉ list_to_set (C:=gset A) (take (Z.to_nat i) keys).
+Proof.
+  intros Hnodup Hlookup Hi_nonneg Hin.
+  rewrite elem_of_list_to_set in Hin.
+  apply list_elem_of_lookup_1 in Hin as [j Htake_lookup].
+  apply lookup_take_Some in Htake_lookup as [Hlookup_j Hj].
+  pose proof (NoDup_lookup _ _ _ _ Hnodup Hlookup_j Hlookup) as ->.
+  lia.
+Qed.
+
+Lemma processed_map_empty `{Countable K} {A} (keys : list K) (m : gmap K A) :
+  processed_map keys 0 m = ∅.
+Proof.
+  apply map_eq. intros key.
+  rewrite /processed_map map_lookup_filter lookup_empty take_0.
+  destruct (m !! key); simpl; [|done].
+  destruct (decide (key ∈ list_to_set (C:=gset K) [])); [|done].
+  rewrite elem_of_list_to_set elem_of_nil in e. done.
+Qed.
+
+Lemma processed_map_lookup_not_current `{Countable K} {A}
+    (keys : list K) i key (m : gmap K A) :
+  NoDup keys →
+  keys !! Z.to_nat i = Some key →
+  (0 ≤ i)%Z →
+  processed_map keys i m !! key = None.
+Proof.
+  intros Hnodup Hlookup Hi_nonneg.
+  rewrite /processed_map. apply map_lookup_filter_None_2. right.
+  intros x Hx Hin. simpl in Hin.
+  exact ((current_key_not_in_take keys i key Hnodup Hlookup Hi_nonneg) Hin).
+Qed.
+
+Lemma processed_map_insert `{Countable K} {A}
+    (keys : list K) i key (m : gmap K A) v :
+  NoDup keys →
+  (0 ≤ i)%Z →
+  keys !! Z.to_nat i = Some key →
+  m !! key = Some v →
+  processed_map keys (i + 1) m = <[key:=v]> (processed_map keys i m).
+Proof.
+  intros Hnodup Hi_nonneg Hkey_lookup Hm_lookup.
+  apply map_eq. intros key'.
+  destruct (decide (key' = key)) as [->|Hne].
+  - rewrite lookup_insert_eq /processed_map.
+    apply map_lookup_filter_Some_2; [done|].
+    simpl.
+    replace (Z.to_nat (i + 1)) with (S (Z.to_nat i)) by lia.
+    rewrite (take_S_r _ _ _ Hkey_lookup).
+    rewrite elem_of_list_to_set elem_of_app /=. right. Timeout 10 set_solver.
+  - replace (<[key:=v]> (processed_map keys i m) !! key') with
+      (processed_map keys i m !! key').
+    2:{ symmetry. apply lookup_insert_ne.
+        intro Heq. apply Hne. symmetry. exact Heq. }
+    assert (Hin_iff : key' ∈ list_to_set (C:=gset K)
+        (take (Z.to_nat (i + 1)) keys) ↔
+      key' ∈ list_to_set (C:=gset K) (take (Z.to_nat i) keys)).
+    { replace (Z.to_nat (i + 1)) with (S (Z.to_nat i)) by lia.
+      rewrite (take_S_r _ _ _ Hkey_lookup).
+      rewrite !elem_of_list_to_set elem_of_app /= elem_of_cons elem_of_nil.
+      split; intros Hin.
+      - destruct Hin as [Hin|Hin]; [done|].
+        destruct Hin as [Heq|[]]. subst. contradiction.
+      - left. done. }
+    destruct (m !! key') as [v'|] eqn:Hm_lookup'.
+    + destruct (decide (key' ∈ list_to_set (C:=gset K)
+        (take (Z.to_nat i) keys))) as [Hin|Hnot].
+      * rewrite /processed_map.
+        transitivity (Some v').
+        -- apply map_lookup_filter_Some_2; [done|].
+           simpl. apply Hin_iff. done.
+        -- symmetry. apply map_lookup_filter_Some_2; [done|done].
+      * rewrite /processed_map.
+        transitivity (@None A).
+        -- apply map_lookup_filter_None_2. right.
+           intros x Hx Hin_succ. simpl in Hin_succ.
+           apply Hnot. apply Hin_iff. done.
+        -- symmetry. apply map_lookup_filter_None_2. right.
+           intros x Hx Hin_old. done.
+    + rewrite /processed_map.
+      transitivity (@None A).
+      * apply map_lookup_filter_None_2. left. done.
+      * symmetry. apply map_lookup_filter_None_2. left. done.
+Qed.
+
+Lemma processed_map_all `{Countable K} {A} (keys : list K) (m : gmap K A) :
+  list_to_set keys = dom m →
+  length keys = size m →
+  processed_map keys (Z.of_nat (size m)) m = m.
+Proof.
+  intros Hdom Hlen. apply map_eq. intros key.
+  destruct (m !! key) as [v|] eqn:Hlookup.
+  - rewrite /processed_map. apply map_lookup_filter_Some_2; [done|].
+    simpl. rewrite Nat2Z.id. replace (size m) with (length keys) by done.
+    replace (take (length keys) keys) with keys
+      by (symmetry; apply take_ge; lia).
+    rewrite Hdom elem_of_dom. eexists. exact Hlookup.
+  - rewrite /processed_map. apply map_lookup_filter_None_2. left. done.
+Qed.
+
 Lemma wp_copyIdentities
     (src : map.t)
     (phys_identities : gmap iammodel.IdentityID.t map.t)
@@ -60,9 +224,133 @@ Lemma wp_copyIdentities
         phys_identities_copy; abs_identities,
         policy_ids_l ↦$ policy_ids)
   }}}.
-(* FIXME: proving this requires map.for_range support for callbacks that use
-   the ranged-over map value. *)
-Proof. Admitted.
+Proof.
+  wp_start as "H".
+  iNamed "H".
+  wp_auto.
+  rewrite exception_do_unseal /exception_do_def.
+  wp_apply wp_map_make1 as "%identities_l Hdst".
+  wp_apply (wp_map_for_range_return_func (key_type:=iammodel.IdentityID)
+    (λ (keys : list iammodel.IdentityID.t) i,
+      ∃ (last_policy_ids_l : map.t) (last_identity : iammodel.IdentityID.t)
+        (dst_phys : gmap iammodel.IdentityID.t map.t),
+        "Hinner" ∷ ([∗ map] policy_ids_l; policy_ids ∈
+          phys_identities; abs_identities, policy_ids_l ↦${dq_inner} policy_ids) ∗
+        "policyIDs" ∷ policyIDs_ptr ↦ last_policy_ids_l ∗
+        "identity" ∷ identity_ptr ↦ last_identity ∗
+        "identities" ∷ identities_ptr ↦ identities_l ∗
+        "Hdst" ∷ identities_l ↦$ dst_phys ∗
+        "Hdst_inner" ∷ ([∗ map] policy_ids_l; policy_ids ∈
+          dst_phys; processed_map keys i abs_identities,
+          policy_ids_l ↦$ policy_ids))%I
+    with "Hsrc").
+  { done. }
+  iIntros (keys) "%Hkeys".
+  iSplitL "Hinner policyIDs identity identities Hdst".
+  { iExists map.nil, (""%go : iammodel.IdentityID.t), ∅. iFrame.
+    rewrite processed_map_empty big_sepM2_empty. done. }
+  iSplitL "".
+  { iModIntro. iIntros (i identity policy_ids_l) "%Hiter Hloop".
+    destruct Hkeys as [Hkeys_dom [Hkeys_len Hkeys_nodup]].
+    destruct Hiter as [Hi_bounds [Hidentity_lookup Hphys_lookup]].
+    destruct Hi_bounds as [Hi_nonneg Hi_upper].
+    iDestruct "Hloop" as (last_policy_ids_l last_identity dst_phys)
+      "(Hinner & policyIDs & identity & identities & Hdst & Hdst_inner)".
+    iDestruct (big_sepM2_dom with "Hinner") as %Hinner_dom.
+    assert (is_Some (abs_identities !! identity)) as [policy_ids Habs_lookup].
+    { apply elem_of_dom. rewrite -Hinner_dom.
+      apply elem_of_dom. eexists. exact Hphys_lookup. }
+    assert (processed_map keys i abs_identities !! identity = None)
+      as Hprocessed_fresh.
+    { apply processed_map_lookup_not_current; done. }
+    iDestruct (big_sepM2_dom with "Hdst_inner") as %Hdst_dom.
+    assert (dst_phys !! identity = None) as Hdst_fresh.
+    { apply not_elem_of_dom. intros Hdst_in.
+      rewrite Hdst_dom in Hdst_in.
+      apply elem_of_dom in Hdst_in as [? Hprocessed_some].
+      rewrite Hprocessed_fresh in Hprocessed_some. done. }
+    assert (processed_map keys (i + 1) abs_identities =
+      <[identity:=policy_ids]> (processed_map keys i abs_identities))
+      as Hprocessed_insert.
+    { apply processed_map_insert; done. }
+    iDestruct (big_sepM2_lookup_acc _ _ _ identity policy_ids_l policy_ids
+      Hphys_lookup Habs_lookup with "Hinner") as "[HpolicyIDs_src Hinner_close]".
+    wp_pures.
+    simpl subst'.
+    wp_auto.
+    wp_apply wp_map_make1 as "%policyIDsCopy_l HpolicyIDsCopy".
+    wp_apply (wp_map_for_range_return_func (key_type:=iammodel.PolicyID)
+      (λ (policy_keys : list iammodel.PolicyID.t) j,
+        ∃ (last_policy_id : iammodel.PolicyID.t) (policy_ids_copy_l : map.t),
+          "policyID" ∷ policyID_ptr ↦ last_policy_id ∗
+          "policyIDsCopy" ∷ policyIDsCopy_ptr ↦ policy_ids_copy_l ∗
+          "HpolicyIDsCopy" ∷ policy_ids_copy_l ↦$
+            processed_map policy_keys j policy_ids)%I
+      with "HpolicyIDs_src").
+    { done. }
+    iIntros (policy_keys) "%Hpolicy_keys".
+    iSplitL "policyID policyIDsCopy HpolicyIDsCopy".
+    { iExists (""%go : iammodel.PolicyID.t), policyIDsCopy_l. iFrame.
+      rewrite processed_map_empty. iFrame. }
+    iSplitL "".
+    { iModIntro. iIntros (j policy_id []) "%Hpolicy_iter Hinner_loop".
+      destruct Hpolicy_keys as [Hpolicy_keys_dom
+        [Hpolicy_keys_len Hpolicy_keys_nodup]].
+      destruct Hpolicy_iter as [Hj_bounds [Hpolicy_key_lookup Hpolicy_lookup]].
+      destruct Hj_bounds as [Hj_nonneg Hj_upper].
+      iDestruct "Hinner_loop" as (last_policy_id policy_ids_copy_l)
+        "(policyID & policyIDsCopy & HpolicyIDsCopy)".
+      wp_pures.
+      simpl subst'.
+      wp_auto.
+      wp_apply (wp_map_insert iammodel.PolicyID with "[$HpolicyIDsCopy]").
+      iIntros "HpolicyIDsCopy". wp_auto.
+      iRight. iSplit; [done|].
+      iExists policy_id, policy_ids_copy_l. iFrame.
+      rewrite -processed_map_insert; done. }
+    iIntros "HpolicyIDs_src Hinner_done".
+    iDestruct "Hinner_done" as (last_policy_id policy_ids_copy_l)
+      "(policyID & policyIDsCopy & HpolicyIDsCopy)".
+    destruct Hpolicy_keys as [Hpolicy_keys_dom
+      [Hpolicy_keys_len Hpolicy_keys_nodup]].
+    rewrite (processed_map_all policy_keys policy_ids
+      Hpolicy_keys_dom Hpolicy_keys_len).
+    iDestruct ("Hinner_close" with "HpolicyIDs_src") as "Hinner".
+    wp_auto.
+    wp_apply (wp_map_insert iammodel.IdentityID with "[$Hdst]").
+    iIntros "Hdst". wp_auto.
+    iAssert (([∗ map] policy_ids_l'; policy_ids' ∈
+      <[identity:=policy_ids_copy_l]> dst_phys;
+      processed_map keys (i + 1) abs_identities,
+      policy_ids_l' ↦$ policy_ids')%I)
+      with "[HpolicyIDsCopy Hdst_inner]" as "Hdst_inner".
+    { rewrite Hprocessed_insert.
+      rewrite (big_sepM2_insert _ dst_phys
+        (processed_map keys i abs_identities)
+        identity policy_ids_copy_l policy_ids Hdst_fresh Hprocessed_fresh).
+      iFrame. }
+    iRight. iSplit; [done|].
+    iExists policy_ids_l, identity, (<[identity:=policy_ids_copy_l]> dst_phys).
+    iFrame. }
+  iIntros "Hsrc Hloop".
+  iDestruct "Hloop" as (last_policy_ids_l last_identity dst_phys)
+    "(Hinner & policyIDs & identity & identities & Hdst & Hdst_inner)".
+  destruct Hkeys as [Hkeys_dom [Hkeys_len Hkeys_nodup]].
+  iDestruct (big_sepM2_dom with "Hinner") as %Hinner_dom.
+  assert (Habs_size : size abs_identities = size phys_identities).
+  { rewrite -(size_dom phys_identities) -(size_dom abs_identities).
+    rewrite Hinner_dom. done. }
+  replace (processed_map keys (Z.of_nat (size phys_identities)) abs_identities)
+    with abs_identities.
+  2:{ rewrite -Habs_size. symmetry. apply processed_map_all.
+      - rewrite Hkeys_dom Hinner_dom. done.
+      - rewrite Habs_size. done. }
+  wp_auto.
+  rewrite return_val_unseal /return_val_def. wp_auto.
+  iApply ("HΦ" $! identities_l dst_phys). iFrame.
+Unshelve.
+  all: unfold iammodel.IdentityID.t, iammodel.PolicyID.t; apply _.
+Qed.
 
 Lemma wp_copyPolicies
     (src : map.t) (policies : gmap iammodel.PolicyID.t iammodel.IdentityPolicy.t) dq :
@@ -72,16 +360,76 @@ Lemma wp_copyPolicies
       "Hsrc" ∷ src ↦${dq} policies ∗
       "Hdst" ∷ dst ↦$ policies
   }}}.
-(* FIXME: proving this requires map.for_range support for callbacks that use
-   the ranged-over map value. *)
-Proof. Admitted.
+Proof.
+  wp_start as "H".
+  iNamed "H".
+  wp_auto.
+  rewrite exception_do_unseal /exception_do_def.
+  wp_apply wp_map_make1 as "%policies_l Hdst".
+  wp_apply (wp_map_for_range_return_func (key_type:=iammodel.PolicyID)
+    (λ (keys : list iammodel.PolicyID.t) i,
+      ∃ (last_policy : iammodel.IdentityPolicy.t)
+        (last_policy_id : iammodel.PolicyID.t),
+        "policy" ∷ policy_ptr ↦ last_policy ∗
+        "policyID" ∷ policyID_ptr ↦ last_policy_id ∗
+        "policies" ∷ policies_ptr ↦ policies_l ∗
+        "Hdst" ∷ policies_l ↦$ processed_map keys i policies)%I
+    with "Hsrc").
+  { done. }
+  iIntros (keys) "%Hkeys".
+  iSplitL "policy policyID policies Hdst".
+  { iExists (zero_val _), (""%go : iammodel.PolicyID.t). iFrame.
+    rewrite processed_map_empty. iFrame. }
+  iSplitL "".
+  { iModIntro. iIntros (i policy_id policy) "%Hiter Hloop".
+    destruct Hkeys as [Hkeys_dom [Hkeys_len Hkeys_nodup]].
+    destruct Hiter as [Hi_bounds [Hpolicy_id_lookup Hpolicy_lookup]].
+    destruct Hi_bounds as [Hi_nonneg Hi_upper].
+    iDestruct "Hloop" as (last_policy last_policy_id)
+      "(policy & policyID & policies & Hdst)".
+    wp_pures.
+    simpl subst'.
+    wp_auto.
+    wp_apply (wp_map_insert iammodel.PolicyID with "[$Hdst]").
+    iIntros "Hdst". wp_auto.
+    iRight. iSplit; [done|].
+    iExists policy, policy_id. iFrame.
+    rewrite -processed_map_insert; done. }
+  iIntros "Hsrc Hloop".
+  iDestruct "Hloop" as (last_policy last_policy_id)
+    "(policy & policyID & policies & Hdst)".
+  destruct Hkeys as [Hkeys_dom [Hkeys_len Hkeys_nodup]].
+  rewrite (processed_map_all keys policies Hkeys_dom Hkeys_len).
+  wp_auto.
+  rewrite return_val_unseal /return_val_def. wp_auto.
+  iApply ("HΦ" $! policies_l). iFrame.
+Unshelve.
+  all: unfold iammodel.PolicyID.t; apply _.
+Qed.
 
 Lemma wp_generatePolicyID :
   {{{ True }}}
     @! iammodel.generatePolicyID #()
   {{{ (policy_id : iammodel.PolicyID.t), RET #policy_id; True }}}.
 Proof.
-Admitted.
+  wp_start as "_".
+  rewrite exception_do_unseal /exception_do_def.
+  wp_bind (@! rand.Int63 #())%E.
+  iApply (wp_rand_Int63 with "[] [HΦ]").
+  { iEval (rewrite is_pkg_init_unfold /=). done. }
+  iNext.
+  iIntros (n) "_".
+  wp_auto.
+  wp_apply (wp_slice_literal (V:=interface.t) (t:=go.any)).
+  iSplitR; first done.
+  iIntros (args) "[Hargs _]". wp_auto.
+  wp_apply (wp_fmt_Sprintf with "[$Hargs]").
+  { iApply is_pkg_init_fmt_trivial. }
+  iIntros (policy_id) "_".
+  wp_auto.
+  rewrite return_val_unseal /return_val_def. wp_auto.
+  iApply "HΦ". done.
+Qed.
 
 Lemma wp_State__generateNewPolicyIDAndUpdate
     l used_policy_ids_l (used_policy_ids : gmap iammodel.PolicyID.t unit) :
